empty message

Isabelle/5. Advanced/Ex5_3.thy
@@ -17,4 +17,130 @@ primrec assoc :: "('key \<times> 'val)list \<Rightarrow> 'key \<Rightarrow> 'val
 "assoc (x#xs) key = (if key=  fst x then Some (snd x) else assoc xs key)"
 
 primrec lookup :: "('a , 'v)trie \<Rightarrow> 'a list \<Rightarrow> 'v option" where 
-"lookup "
+"lookup t [] = value t"|
+"lookup t (x#xs) = (case assoc (alist t) x of
+  None \<Rightarrow> None | 
+  Some newT \<Rightarrow> lookup newT xs)"
+
+primrec update :: "('a , 'v) trie \<Rightarrow> 'a list \<Rightarrow> 'v \<Rightarrow> ('a , 'v)trie" where
+"update t [] val =  Trie (Some val) (alist t)"|
+"update t (x#xs) val = (case assoc (alist t) x of
+  None \<Rightarrow> Trie (value t) ((x , update (Trie None []) xs val) # alist t)|
+  Some v \<Rightarrow> Trie  (value t) ((x , update v xs val) # alist t))"
+
+lemma empty_tree_lookup : "lookup (Trie None []) ls = None" by (induction ls ; simp)
+
+theorem "\<forall> t v bs. lookup (update t as v) bs = (if as = bs then Some v else lookup t bs)" 
+proof (induction as)
+  case Nil
+  then show ?case 
+  proof - 
+    {
+      fix t::"('a , 'v)trie"
+      fix v bs
+      have "lookup (update t [] v) bs = (if [] = bs then Some v else lookup t bs)" 
+      proof (cases "bs")
+        case Nil
+        then show ?thesis by simp
+      next
+        case (Cons a list)
+        then show ?thesis by simp
+      qed
+    }
+    thus ?thesis by blast
+  qed
+next
+  case (Cons a as)
+  assume hyp:"\<forall>(t::('a,'v)trie) v bs. lookup (update t as v) bs = (if as = bs then Some v else lookup t bs)"
+  then show " \<forall>(t::('a,'v)trie) v bs. lookup (update t (a # as) v) bs = (if a # as = bs then Some v else lookup t bs)"
+  proof -
+    {
+      fix t::"('a , 'v)trie"
+      fix bs v
+     
+      have "lookup (update t (a # as) v) bs = (if a # as = bs then Some v else lookup t bs) " 
+      proof (cases "bs")
+        case Nil
+        then show ?thesis by (cases "assoc (alist t) a" ; simp)
+      next
+        case (Cons aa list)
+        assume c1:"bs = aa # list"
+        then show ?thesis 
+        proof (cases "assoc (alist t) a")
+          case None
+          then show ?thesis 
+          proof (cases "a = aa")
+            case True
+            from hyp have tmp:"lookup (update (Trie None []) as v) list = (if as = list then Some v else lookup (Trie None []) list) " by simp
+
+            have "lookup (update t (a # as) v) bs = lookup  (Trie (value t) ((a , update (Trie None []) as v) # alist t)) bs" using None by simp
+            also have "\<dots> = lookup (update (Trie None []) as v) list" using c1 True None by simp
+            also have "\<dots> = (if as = list then Some v else lookup (Trie None []) list)" using tmp by simp
+            also have "\<dots> = (if a # as = bs then Some v else lookup (Trie None []) list)" using True c1 by simp
+            also have "\<dots> = (if a # as = bs then Some v else lookup t bs)" using empty_tree_lookup c1 True None by auto
+            finally show ?thesis by assumption
+          next
+            case False
+            let ?tmp="update (Trie None []) as v"
+            
+            have "lookup (update t (a # as) v) bs = lookup (Trie (value t) ((a , ?tmp )  # alist t)) bs" using None by simp
+            also have "\<dots> = lookup t bs" using False c1 by simp
+            finally show ?thesis using c1 False by simp
+          qed
+        next
+          case (Some aaa)
+          then show ?thesis using c1 hyp by (cases "a = aa" ; simp)
+        qed
+      qed
+    }
+    then show " \<forall>(t::('a,'v)trie) v bs. lookup (update t (a # as) v) bs = (if a # as = bs then Some v else lookup t bs)"  by simp
+  qed
+qed
+
+primrec modify :: "('a , 'v)trie \<Rightarrow> 'a list \<Rightarrow> 'v option \<Rightarrow> ('a , 'v)trie" where 
+"modify t [] v = Trie v (alist t)"|
+"modify t (x#xs) v = (let tr  = (case assoc (alist t) x of
+  None \<Rightarrow>  (x ,modify (Trie None []) xs v)   |
+  Some t2 \<Rightarrow>  (x , modify t2 xs v)  ) 
+  in Trie (value t) (tr # alist t))"
+
+theorem "\<forall> t v bs. lookup (modify t as v) bs = (if as = bs then v else lookup t bs)" 
+proof (induction as)
+case Nil
+  then show ?case  using alist.simps  modify.simps(1) list.exhaust  lookup.simps  value.simps by metis
+next
+  case (Cons a as)
+  assume hyp:"\<forall>(t::('a,'v)trie) (v::'v option) (bs::'a list). lookup (modify t as v) bs = (if as = bs then v else lookup t bs)"
+  {
+    fix t::"('a , 'v) trie"
+    fix v bs
+    have "lookup (modify t (a # as) v) bs = (if a # as = bs then v else lookup t bs)" 
+    proof (cases bs)
+      case Nil
+      then show ?thesis by simp
+    next
+      case (Cons aa list)
+      show ?thesis 
+      proof (cases "assoc (alist t) a")
+        case None
+        from hyp have tmp:"lookup (modify (Trie None []) (as::'a list) v) (list :: 'a list) = (if as = list then v else lookup (Trie None []) list)" by simp
+        then show ?thesis using Cons hyp None 
+        proof (cases "a = aa")
+          case True
+          have "lookup (modify t (a # as) v) bs = lookup  (modify (Trie None []) as v) list" using None Cons True  by simp
+          also have "\<dots> = (if as = list then v else lookup (Trie None []) list)" using tmp by simp
+          also have "\<dots> = (if a#as = bs then v else lookup t bs)" using Cons True None empty_tree_lookup by auto
+          finally show ?thesis by assumption
+        next
+          case False
+          then show ?thesis using Cons hyp None by simp
+        qed
+      next
+        case (Some aaa)
+        then show ?thesis using hyp Cons by (cases "a = aa" ; simp)
+      qed
+    qed
+  }
+  then show "\<forall>(t::('a,'v)trie) (v::'v option) bs. lookup (modify t (a # as) v) bs = (if a # as = bs then v else lookup t bs)" by simp
+qed
+
