Isabelle_ZF/Ex1_2.thy
@@ -1,0 +1,16 @@
+theory Ex1_2 
+  imports ZF
+begin 
+
+
+consts 
+  replace :: "i \<Rightarrow> i \<Rightarrow> i \<Rightarrow> i"
+
+
+notation 
+  Cons (infix "$$" 55)
+
+primrec 
+"replace (old, new, []) = []"
+"replace (old ,new, x$$xs) = (if (old = x) then new  else x) $$ replace(old,new,xs)"
+
